Refactor

HoareTactics/reduce.v
@@ -1,10 +1,6 @@
 Require Import GPUCSL scan_lib LibTactics Psatz CSLLemma SetoidClass.
 Require Import CSLLemma CSLTactics.
 
-Coercion Var : string >-> var.
-Open Scope string_scope.
-Open Scope list_scope.
-
 Arguments div _ _ : simpl never.
 Arguments modulo _ _ : simpl never.
 
@@ -496,7 +492,7 @@ Definition jth_pre :=
       "inp" |-> inp ::
       "out" |-> out ::
       "l" |-> Zn (Datatypes.length init_vals) ::
-      "bid" |-> Zn (nf bid) :: nil)).
+      nil)).
 
 Definition jth_post :=
   Ex sh_vals,
@@ -521,535 +517,9 @@ Definition E := fun x =>
   else if var_eq_dec x "d" then Lo
   else Hi.
 
-Require Import Skel_lemma scan_lib.
-
-Ltac no_side_cond tac :=
-  (now tac) || (tac; [now auto_star..|idtac]).
-
-Lemma fv_edenot e s s' :
-  (forall x, In x (fv_E e) -> s x = s' x)
-  -> edenot e s = edenot e s'.
-Proof.
-  intros Heq.
-  Ltac tac Heq H := rewrites* H; try now (intros; applys* Heq; repeat rewrite in_app_iff; eauto).
-  induction e; simpl in *; 
-  (try no_side_cond ltac:(tac Heq IHe));
-  (try no_side_cond ltac:(tac Heq IHe1));
-  (try no_side_cond ltac:(tac Heq IHe2)); try congruence.
-  rewrites* Heq.
-Qed.
-
-Lemma low_assn_vars R P Env E :
-  (forall e x v, In (e |-> v) Env -> In x (fv_E e) -> E x = Lo) ->
-  low_assn E (Assn R P Env).
-Proof.
-  intros HEnv.
-  unfold low_assn, Bdiv.low_assn, Bdiv.indeP; simpl.
-  unfold low_eq.
-  unfold Assn; split; intros Hsat; sep_split_in Hsat; sep_split; eauto;
-  induction Env as [|[? ?] ?]; simpl in *; eauto; destruct HP0; split;
-  unfold_conn_all; simpl in *; eauto;
-  [rewrites (>>fv_edenot s1); [|eauto];
-   intros; rewrites* H..].
-Qed.
-
-Lemma low_assn_ex {T : Type} G (P : T -> assn) :
-  (forall x, low_assn G (P x)) ->
-  low_assn G (Ex x, P x).
-Proof.
-  unfold low_assn, Bdiv.low_assn, Bdiv.indeP.
-  intros Hl s1 s2 h Hlow; simpl.
-  split; intros [x H]; exists x; simpl in *.
-  rewrite Hl.
-  exact H.
-  apply Bdiv.low_eq_sym; eauto.
-  rewrite Hl.
-  exact H.
-  eauto.
-Qed.
-
-Lemma low_assn_FalseP E : low_assn E FalseP.
-Proof.
-  intros s1 s2 h H; tauto.
-Qed.
-Ltac des H :=
-  let t := type of H in idtac "H : " t;
-  match type of H with
-  | _ \/ _ =>
-    let H' := fresh "H" in
-    destruct H as [H | H']; [des H | des H']
-  | (_ |-> _ = _ |-> _) => inverts H; substs
-  | False => destruct H
-  | _ => substs
-  end.
-Ltac prove_low_expr :=
-  let H1 := fresh "H" in
-  let H2 := fresh "H" in
-  simpl in *; 
-  intros ? ? ? H1 H2;
-  des H1; simpl in *; des H2; simpl; eauto.
-
-Ltac prove_low_assn :=
-  lazymatch goal with
-  | [|- low_assn _ (Ex _ : _, _) ] =>
-    apply low_assn_ex; intros ?; prove_low_assn
-  | [|- low_assn _ (Assn _ _ _)] =>
-    apply low_assn_vars; prove_low_expr
-  | [|- low_assn _ FalseP] =>
-    apply low_assn_FalseP
-  end.
-
-Lemma rule_block n BS E (Ps Qs : Vector.t assn n) (P : assn) c (Q : assn) ty:
-  n <> 0 ->
-  (forall i : nat,
-      (forall tid : Fin.t n, low_assn E (Vector.nth (fst (BS i)) tid)) /\
-      (forall tid : Fin.t n, low_assn E (Vector.nth (snd (BS i)) tid))) ->
-  (forall (i : nat),
-      Bdiv.Aistar_v (fst (BS i)) |= Bdiv.Aistar_v (snd (BS i))) ->
-  (forall (i : nat) (tid : Fin.t n),
-      precise (Vector.nth (fst (BS i)) tid) /\
-      precise (Vector.nth (snd (BS i)) tid)) ->
-  P |= Bdiv.Aistar_v Ps ->
-  Bdiv.Aistar_v Qs |= Q ->
-  (forall tid : Fin.t n, low_assn E (Vector.nth Ps tid)) ->
-  (forall tid : Fin.t n, low_assn E (Vector.nth Qs tid)) ->
-  typing_cmd E c ty ->
-  (forall tid : Fin.t n,
-      CSL BS tid (Vector.nth Ps tid ** !("tid" === Zn (nf tid))) c
-          (Vector.nth Qs tid)) -> CSLp n E P c Q.
-Proof.
-  intros; eapply rule_par; eauto.
-  destruct n; try omega; eauto.
-  intros ? [? ?] ?; simpl in *; unfold sat in *; eauto.
-Qed.
-
-Lemma rule_conseq (n : nat)
-  (bspec : nat -> Vector.t assn n * Vector.t assn n)
-  (tid : Fin.t n) (P : assn) (C : cmd) (Q P' Q' : assn) :
-  CSL bspec tid P C Q -> P' |= P -> Q |= Q' -> CSL bspec tid P' C Q'.
-Proof.
-  intros; eapply rule_conseq; eauto.
-Qed.
-
-Lemma assn_var_in Res P Env x (v : val) :
-  (Assn Res P Env ** !(x === v)) == (Assn Res P (x |-> v :: Env)).
-Proof.
-  unfold Assn; split; simpl; intros H; sep_split_in H; sep_split; eauto.
-  split; eauto.
-  destruct HP0; eauto.
-  destruct HP0; eauto.
-Qed.
-
-Definition istar ls := List.fold_right Star Emp ls.
-
-Lemma conj_xs_assn st n Res P Env :
-  n <> 0 ->
-  conj_xs (ls_init st n (fun i => Assn (Res i) P Env)) ==
-  Assn (istar (ls_init st n (fun i => Res i))) P Env.
-Proof.
-  unfold Assn, sat; intros Hn0 s h.
-  split; intros.
-  - repeat sep_rewrite_in @ls_star H.
-    repeat sep_rewrite_in @ls_pure H; sep_split_in H.
-    apply (ls_emp _ _ 0) in HP; rewrite ls_init_spec in HP.
-    destruct lt_dec; try omega.
-    apply (ls_emp _ _ 0) in HP0; rewrite ls_init_spec in HP0.
-    destruct lt_dec; try omega.
-    sep_split; eauto.
-    Lemma conj_xs_istar s n f :
-      res_denote (istar (ls_init s n f)) == conj_xs (ls_init s n (fun i => res_denote (f i))).
-    Proof.
-      revert s; induction n; simpl.
-      - reflexivity.
-      - intros; rewrite IHn; reflexivity.
-    Qed.
-    fold_sat; rewrite conj_xs_istar; apply H.
-  - sep_split_in H.
-    repeat sep_rewrite @ls_star.
-    repeat sep_rewrite @ls_pure; sep_split.
-    + apply ls_emp'; intros i; rewrite init_length, ls_init_spec; intros;
-      destruct lt_dec; try omega; eauto.
-    + apply ls_emp'; intros i; rewrite init_length, ls_init_spec; intros;
-      destruct lt_dec; try omega; eauto.
-    + fold_sat; rewrite <-conj_xs_istar; apply H.
-Qed.
-
-Lemma sc_v2l n (assns : Vector.t assn n) :
-  Bdiv.Aistar_v assns == conj_xs (Vector.to_list assns).
-Proof.
-  simpl; introv; apply sc_v2l.
-Qed.
-
-Lemma emp_unit_l P: 
-  (Emp *** P) == P.
-Proof.
-  intros s h; unfold sat_res; simpl.
-  apply emp_unit_l.
-Qed.
-
-Lemma emp_unit_r P: 
-  (P *** Emp) == P.
-Proof.
-  intros s h; unfold sat_res; simpl.
-  apply emp_unit_r.
-Qed.
-
-Lemma init_emp_emp b n :
-  istar (ls_init b n (fun _ => Emp)) == Emp.
-Proof.
-  revert b; induction n; simpl; [reflexivity|]; intros.
-  rewrite IHn.
-  rewrite emp_unit_l; reflexivity.
-Qed.
-
-Lemma ls_star b n P Q :
-  istar (ls_init b n (fun i => P i *** Q i)) ==
-  (istar (ls_init b n (fun i => P i)) *** istar (ls_init b n (fun i => Q i))).
-Proof.
-   revert b; induction n; simpl; eauto.
-   - intros; rewrite emp_unit_l; reflexivity.
-   - intros; rewrite IHn; rewrite <-!res_assoc.
-     apply res_star_proper; [reflexivity|].
-     rewrite res_CA; reflexivity.
-Qed.
-
-Lemma istar_app Ps Qs: 
-  istar (Ps ++ Qs) == (istar Ps *** istar Qs).
-Proof.
-  induction Ps; simpl; eauto.
-  rewrite emp_unit_l; reflexivity.
-  rewrite IHPs, <-res_assoc; reflexivity.
-Qed.  
-                       
-Lemma array'_ok n ptr dist vals s p :
-  (forall i, s <= i < length vals + s -> dist i < n) ->
-  istar (ls_init 0 n (fun i => array' ptr (ith_vals dist vals i s) p)) ==
-  array ptr vals p.
-Proof.
-  revert s ptr; induction vals; intros; simpl.
-  - intros s' h.
-    rewrite init_emp_emp; reflexivity.
-  - rewrite ls_star.
-    rewrite IHvals.
-    apply res_star_proper; try reflexivity.
-    lazymatch goal with
-    | [|- context [ls_init 0 n ?f]] =>
-      cutrewrite (ls_init 0 n f =
-                  (ls_init 0 (dist s) (fun _ => Emp) ++
-                  (ptr |->p (p, a)) ::
-                  ls_init ((dist s) + 1) (n - dist s - 1) (fun _ => Emp)))
-    end.
-    rewrite istar_app, init_emp_emp; simpl; rewrite init_emp_emp.
-    rewrite emp_unit_l, emp_unit_r; reflexivity.
-    specialize (H s).
-    simpl in *.
-    cutrewrite (n = (dist s) + 1 + (n - dist s - 1)); [|omega].
-    repeat rewrite ls_init_app; simpl.
-    rewrite <-app_assoc; simpl.
-    f_equal; [apply ls_init_eq'|f_equal]; eauto.
-    intros; simpl; destruct Nat.eq_dec; try omega; eauto.
-    intros; simpl; destruct Nat.eq_dec; try omega; eauto.
-    lazymatch goal with
-    | [|- _ _ ?p _ = _ _ ?q _] =>
-      cutrewrite (q = p); [|lia];
-      apply ls_init_eq';
-      intros; simpl; destruct Nat.eq_dec; try omega; eauto
-    end.
-    intros; apply H; simpl; omega.
-Qed.
-
-Lemma nseq_nth_same T i n (x : T) :
-  nth i (nseq n x) x = x.
-Proof.
-  rewrite nth_nseq; destruct leb; auto.
-Qed.
-
-Lemma ex_assn_in_env (x : var) v Res P Env s h n :
-  sat s h (conj_xs (ls_init 0 n (fun i => Assn (Res i) (P i) (Env i)))) ->
-  (forall i, i < n -> evalExp (Env i) x (Zn (v i))) -> 
-  exists c, forall i, i < n -> v i = c.
-Proof.
-  unfold sat, Assn; intros H Hin.
-  repeat sep_rewrite_in @scan_lib.ls_star H;
-  repeat sep_rewrite_in @ls_pure H; sep_split_in H.
-  exists (Z.to_nat (s x)).
-  intros i Hi.
-  eapply (ls_emp _ _ i) in HP0; rewrite ls_init_spec in HP0.
-  destruct lt_dec; try omega.
-  simpl in HP0.
-  forwards*: (>>evalExp_ok (Env i)).
-  unfold_conn_in H0; simpl in *.
-  rewrite H0, Nat2Z.id; auto.
-Qed.
-
-Ltac find_const fs H :=
-  let find v :=
-    match goal with _ => idtac end; 
-    lazymatch type of H with
-    | sat ?s ?h (conj_xs (ls_init 0 ?n (fun i => Assn (@?Res i) (@?P i) (@?Env i)))) =>
-      idtac Res P Env;
-        let x := fresh "x" in
-        let Heq := fresh "Heq" in
-        evar (x : var);
-        forwards [? Heq]: (ex_assn_in_env x (fun i => nth i v 0) Res P Env s h n H);
-        unfold x in *;
-        [now (intros; evalExp) |
-         repeat (erewrite ls_init_eq0 in H; [|intros; rewrite Heq; eauto; reflexivity])]
-  end in
-  let rec iter fs :=
-      lazymatch fs with
-      | (?x, ?y) =>
-        find x;
-        iter y
-      | ?x => idtac 
-      end in
-  iter fs.
-
-Ltac dest_ex_in acc H :=
-  match goal with _ => idtac end;
-  lazymatch type of H with
-  | sat _ _ (conj_xs (ls_init 0 ?n (fun i => Ex t : ?T, @?P i t))) =>
-    let d := default T in
-    rewrite (ls_exists0 d) in H; destruct H as [t H];
-    sep_split_in H; unfold_pures; fold_sat_in H; dest_ex_in (t, acc) H
-  | sat _ _ (conj_xs (ls_init 0 ?n (fun i => Assn (@?Res i) (@?P i) (@?Env i)))) =>
-    find_const acc H
-  end.
-
-Ltac dest_ex :=
-  repeat (lazymatch goal with
-  | [|- sat _ _ (conj_xs (ls_init 0 ?n (fun i => Ex x : ?T, @?P i x)))] =>
-    let x := fresh "x" in
-    evar (x : T);
-    rewrite (ls_exists0 x);
-    eexists (nseq n x); unfold x; sep_split;
-    [rewrite length_nseq; reflexivity|]; fold_sat;
-    erewrite @ls_init_eq0; [|intros; rewrite nseq_nth_same; reflexivity]
-  end).
-
-Ltac prove_istar_imp :=
-  let s := fresh "s" in
-  let h := fresh "h" in
-  let H := fresh "H" in
-  let simplify :=
-      let i := fresh "i" in
-      let Hi := fresh in
-      let Hex := fresh in
-      let Heq := fresh in
-      intros i Hi;
-        lazymatch goal with
-          [|- match ?X with inleft _ => _ | inright _ => _ end = _] =>
-          destruct X as [|Hex] eqn:Heq; [|destruct Hex; omega]
-        end;
-        rewrite (Fin_nat_inv Heq); reflexivity in
-  intros s h H;
-  match goal with _ => idtac end;
-  try lazymatch type of H with
-  | sat _ _ (Bdiv.Aistar_v (MyVector.init _))  =>
-    rewrite sc_v2l, (vec_to_list_init0 _ emp) in H;
-    erewrite ls_init_eq0 in H; [|simplify];
-    dest_ex_in tt H;
-    rewrite conj_xs_assn in H; auto
-  end;
-  try lazymatch goal with
-  | [|- sat _ _ (Bdiv.Aistar_v (MyVector.init _)) ] =>
-    rewrite sc_v2l, (vec_to_list_init0 _ emp);
-    erewrite ls_init_eq0; [|simplify];
-    dest_ex;
-    rewrite conj_xs_assn; auto
-  end;
-  revert s h H; prove_imp.
-
-
-Ltac ls_rewrite_in Heq H :=
-  erewrite ls_init_eq0 in H; [|intros; rewrite Heq; reflexivity].
-
-Lemma precise_false : precise (fun _ _ => False).
-Proof.
-  unfold precise; intros; tauto.
-Qed.
-
-Lemma precise_sat (P Q : assn) :
-  (Q |= P) -> precise P -> precise Q.
-Proof.
-  unfold precise; simpl; intros Hsat HprecP; introv.
-  intros HsatQ HsatQ' ? ? ?.
-  eapply HprecP; eauto; apply Hsat; eauto.
-Qed.
-
-Definition precise_res P :=
-  forall (h1 h2 h1' h2' : pheap) s,
-    sat_res s h1 P ->
-    sat_res s h2 P ->
-    pdisj h1 h1' ->
-    pdisj h2 h2' ->
-    phplus h1 h1' = phplus h2 h2' -> h1 = h2. 
-
-Lemma precise_assn Res P Env :
-  precise_res Res
-  -> precise (Assn Res P Env).
-Proof.
-  unfold Assn; intros.
-  eapply precise_sat; unfold sat; intros s h Hsat; sep_split_in Hsat; eauto.
-Qed.
-
-Lemma precise_star (P Q : res) : precise_res P -> precise_res Q -> precise_res (P *** Q).
-Proof.
-  unfold_conn; intros pp pq h1 h2 h1' h2' s hsat hsat' hdis hdis' heq; simpl in *.
-  destruct hsat as [ph1 [ph1' [satp1 [satq1 [Hdis1 Heq1]]]]], 
-                   hsat' as [ph2 [ph2' [satp2 [satq2 [Hdis2 Heq2]]]]].
-  destruct h1 as [h1 ?], h2 as [h2 ?]; apply pheap_eq; simpl in *; rewrite <-Heq1, <-Heq2 in *.
-  apply pdisj_padd_expand in hdis; apply pdisj_padd_expand in hdis'; eauto.
-  rewrite !padd_assoc in heq; try tauto. 
-  f_equal; destruct hdis as [hdis1 hdis2], hdis' as [hdis1' hdis2'].
-  - rewrite (pp ph1 ph2 (phplus_pheap hdis2) (phplus_pheap hdis2') s); eauto.
-  - rewrite padd_left_comm in heq at 1; try tauto.
-    rewrite (@padd_left_comm _ ph2 ph2' h2') in heq; try tauto.
-    pose proof (pdisjE2 hdis1 hdis2) as dis12; pose proof (pdisjE2 hdis1' hdis2') as dis12'.
-    rewrite (pq ph1' ph2' (phplus_pheap dis12) (phplus_pheap dis12') s); simpl in *; eauto; 
-    apply pdisj_padd_comm; eauto.
-Qed.
-
-Lemma precise_mps l v p :
-  precise_res (l |->p (p, v)).
-Proof.
-  unfold precise_res, precise; intros; simpl in *.
-  unfold sat_res in *; simpl in *; unfold_conn_all; simpl in *.
-  destruct h1 as [h1 ?], h2 as [h2 ?]; apply pheap_eq.
-  extensionality x; simpl in *; rewrite H, H0; auto.
-Qed.
-
-Lemma precise_emp :
-  precise_res Emp.
-Proof.
-  unfold precise_res, sat_res, sat; simpl.
-  intros; applys precise_emp; simpl; eauto.
-Qed.
-
-Hint Resolve precise_star precise_mps precise_emp precise_false precise_assn.
-
-Lemma precise_array l vs p: 
-  precise_res (array l vs p).
-Proof.
-  revert l; induction vs; simpl; eauto.
-Qed.
-
-Lemma precise_array' l vs q :
-  precise_res (array' l vs q).
-Proof.
-  revert l; induction vs as [|[?|] ?]; simpl; eauto.
-Qed.              
-
-Hint Resolve precise_star precise_array precise_array'.
-
-Lemma ty_var' g v ty :
-  g v = ty -> typing_exp g v ty.
-Proof.
-  intros; constructor; rewrite H; destruct ty; eauto.
-Qed.
-Ltac prove_typing_exp :=
-  lazymatch goal with
-  | |- typing_exp ?E (Evar ?v) _ => apply ty_var'; simpl; eauto
-  | |- typing_exp ?E (Enum _) _ => apply (ty_num _ _ Lo)
-  | |- typing_exp ?E (_ ?e1 ?e2) _ => constructor; prove_typing_exp
-  | |- typing_exp ?E (_ ?e) _ => constructor; prove_typing_exp
-  end.
-Ltac prove_typing_lexp :=
-  match goal with |- ?g => idtac g end;
-  lazymatch goal with
-  | |- typing_lexp _ (Sh ?e) _ =>
-    idtac "A";
-    constructor; prove_typing_exp
-  | |- typing_lexp _ (Gl ?e) _ =>
-    idtac "A";
-    constructor; prove_typing_exp
-  | |- typing_lexp _ (_ +o _) _ =>
-    idtac "B";
-    constructor; [prove_typing_lexp | prove_typing_exp]; simpl
-  end.
-Ltac prove_typing_bexp :=
-  match goal with |- ?g => idtac g end;
-  lazymatch goal with
-  | |- typing_bexp _ (Beq _ _) _ =>
-    constructor; prove_typing_exp; simpl
-  | |- typing_bexp _ (_ <C _) _ =>
-    constructor; prove_typing_exp; simpl
-  | |- typing_bexp _ (Bnot _) _ =>
-    idtac "A";
-    constructor; prove_typing_bexp
-  | |- typing_lexp _ (Band _ _) _ =>
-    idtac "B";
-    constructor; [prove_typing_bexp | prove_typing_bexp]; simpl
-  end.
-
-Lemma le_type_hi ty : 
-  le_type ty Hi = true.
-Proof.
-  destruct ty; auto.
-Qed.
-
-Ltac prove_le_type :=
-  eauto;
-  lazymatch goal with
-  | [|- le_type Lo _ = true] => eauto
-  | [|- le_type _ Hi = true] => apply le_type_hi
-  | _ => idtac
-  end.
-
-Ltac prove_typing_cmd :=
-  lazymatch goal with
-  | [|- typing_cmd _ (_ ::T _ ::= [_]) _] =>
-    eapply ty_read; simpl; [prove_typing_lexp | prove_le_type]
-  | [|- typing_cmd _ (_ ::T _ ::= _) _] =>
-    eapply ty_assign; simpl; [prove_typing_exp | prove_le_type]
-  | [|- typing_cmd _ ([_] ::= _) _] => constructor
-  | [|- typing_cmd _ (_ ;; _) _] => constructor
-  | [|- typing_cmd _ (BARRIER (_) ) _] => constructor
-  | [|- typing_cmd _ (Cwhile _ _) _ ] => econstructor; [prove_typing_bexp| ]
-  | [|- typing_cmd _ (WhileI _ _ _) _ ] => econstructor; [prove_typing_bexp| ]
-  | [|- typing_cmd _ (Cif _ _ _) _ ] => econstructor; [prove_typing_bexp|..]
-  | [|- typing_cmd _ Cskip _ ] => constructor
-  | _ => idtac
-  end.
-
-Lemma precise_ex T (P : T -> assn) :
-  (forall x, precise (P x)) ->
-  (forall x1 x2 s h1 h2, sat s h1 (P x1) -> sat s h2 (P x2) -> x1 = x2) ->
-  precise (Ex x, (P x)).
-Proof.
-  unfold precise; simpl; intros Hprec Heqx; introv [x Hsat] [x' Hsat'] Hdisj Hdisj' Heqh.
-  rewrites (Heqx x x' s h1 h1') in Hsat; auto.
-  eapply Hprec; eauto.
-Qed.
-
-Lemma eval_to_Zn_unique s h Res P Env (x : exp) v :
-  sat s h (Assn Res P Env) -> 
-  evalExp Env x (Zn v) -> 
-  v = Z.to_nat (edenot x s).
-Proof.
-  intros.
-  unfold Assn, sat in *; sep_split_in H.
-  forwards*: (>>evalExp_ok); unfold_pures.
-  rewrite H1, Nat2Z.id; auto.
-Qed.
-
-Ltac prove_uniq := match goal with
-| [H : context [?x |-> Zn ?v1], H' : context [?y |-> Zn ?v2] |- ?v1 = ?v2] =>
-  forwards*: (>>eval_to_Zn_unique x v1 H); [evalExp|];
-  forwards*: (>>eval_to_Zn_unique y v2 H'); [evalExp|];
-  congruence
-end.
-
-Ltac prove_precise :=
-  match goal with
-  | [|- precise (Ex _, _)] =>
-    apply precise_ex; [intros; eauto| intros; prove_uniq]
-  | [|- _] => eauto
-  end.
-
 Lemma reduce_ok_b :
   CSLp ntrd E
-       jth_pre
+       (jth_pre ** !("bid" === Zn (nf bid)))
        (reduce TrueP)
        jth_post.
 Proof.
@@ -1067,6 +537,7 @@ Proof.
     unfold dist; repeat destruct lt_dec; try omega.
   - unfold BS; intros [|[|i]] ?; simpl; rewrite !MyVector.init_spec; split; prove_precise.
   - unfold jth_pre, ith_pre.
+    intros s h H; rewrite assn_var_in in H; revert s h H; 
     prove_istar_imp.
     repeat rewrite ls_star.
     rewrite array'_ok; [|intros; lia]; auto.
@@ -1088,3 +559,44 @@ Proof.
 Qed.
    
 End block.
+
+Definition reduce_prog := Pr ((SD "arr" Int ntrd) :: nil) (reduce TrueP).
+
+Lemma rule_p_conseq (P P' : assn) (n : nat) (E : env) (C : cmd) (Q Q' : assn) :
+  CSLp n E P C Q -> P' |= P -> Q |= Q' -> CSLp n E P' C Q'.
+Proof.
+  intros.
+  eapply CSLp_backward; [eapply CSLp_forward|]; eauto.
+Qed.
+
+Lemma reduce_ok_g :
+  CSLg ntrd nblk
+       (Assn (array (SLoc arr) sh_vals 1 ***
+              array (GLoc inp) init_vals 1 ***
+              array (GLoc out) out_vals 1)
+             True
+             ("arr" |-> arr ::
+              "inp" |-> inp ::
+              "out" |-> out ::
+              "l" |-> Zn (length init_vals) :: nil))
+       reduce_prog
+       (Assn (array (SLoc arr) sh_vals 1 ***
+              array (GLoc inp) init_vals 1 ***
+              array (GLoc out) (ls_init 0 nblk (fun i => reduce.sum_of (reg_b' i))) 1)
+             True
+             nil).
+Proof.
+  applys (>> rule_grid E (MyVector.init jth_pre) (MyVector.init jth_post));
+  unfold jth_pre, jth_post, E; eauto.
+  - admit.
+  - intros; eapply rule_p_conseq; eauto using (reduce_ok_b bid);
+    admit.
+  - admit.
+  -  
+  - admit.
+  - admit.
+  - admit.
+  - admit.
+  - admit.
+  - admit.
+Qed.
